\documentclass[12pt]{article}
\usepackage{geometry,amsmath,amssymb, graphicx, natbib, float, enumerate}
\geometry{margin=1in}
\renewcommand{\familydefault}{cmss}
\restylefloat{table}
\restylefloat{figure}

\newcommand{\code}[1]{\texttt{#1}}
\newcommand{\Var}{\mathrm{Var}}
\newcommand{\logit}{\mathrm{logit}}

\begin{document}
\noindent {\bf Lecture 1 Homework. Basic prerequisites, use any resource that you'd like}
\begin{enumerate}[1.]
\item Prove DeMorgan's laws. That is, that $(A \cup B ) ^c = A^c \cap B^c$ and $(A \cap B) ^ c = A^c \cup B^c$.
\item Prove that $(A^c)^c = A$.
\item Prove that $(A \cup B) \cap C = (A\cap C) \cup (B\cap C)$.
\item Show that the function $\frac{1}{\beta} \exp(-x / \beta)$ integrates to $1$ over $x > 0$ for $\beta > 0$.
\item Show that the function $\frac{e^{-x}}{\left(1+  e^{-x} \right)^2}$ integrates to $1$ over $-\infty < x < \infty$.
\item Show that the derivative of the function $(1 + e^{-x})^{-1}$ is the function from the previous problem.
\item Plot the functions from the previous 3 problems in R.
\item Argue that $\sum_{x=0}^\infty \frac{e^{-\lambda}\lambda^x}{x!} = 1$ for $\lambda > 0$.
\item Argue that $\sum_{x=0}^\infty p(1 - p)^{x-1} = 1$ 
\end{enumerate}
\end{document}
